WIP

FallDecoupled.v
@@ -28,10 +28,10 @@ Section FallDecoupled.
   | Even_rise (A : even) : transitions_FD
   | Odd_fall  (B : odd) : transitions_FD
   | Odd_rise  (B : odd) : transitions_FD
-  | Even_rise_odd_rise (E : even) (O : odd) : In (E,O) (even_odd_neighbors c) -> transitions_FD (* E+ → O+ *)
-  | Odd_fall_even_rise (E : even) (O : odd) : In (E,O) (even_odd_neighbors c) -> transitions_FD (* O- → E+ *)
-  | Odd_rise_even_rise (O : odd) (E : even) : In (O,E) (odd_even_neighbors c) -> transitions_FD (* O+ → E+ *)
-  | Even_fall_odd_rise (O : odd) (E : even) : In (O,E) (odd_even_neighbors c) -> transitions_FD (* E- → O+ *)
+  | Even_rise_odd_rise (E : even) (O : odd) : (*In (E,O) (even_odd_neighbors c) ->*) transitions_FD (* E+ → O+ *)
+  | Odd_fall_even_rise (E : even) (O : odd) : (*In (E,O) (even_odd_neighbors c) ->*) transitions_FD (* O- → E+ *)
+  | Odd_rise_even_rise (O : odd) (E : even) : (*In (O,E) (odd_even_neighbors c) ->*) transitions_FD (* O+ → E+ *)
+  | Even_fall_odd_rise (O : odd) (E : even) : (*In (O,E) (odd_even_neighbors c) ->*) transitions_FD (* E- → O+ *)
   .
   Instance eqdecFD : eq_dec transitions_FD.
   Proof.
@@ -44,34 +44,465 @@ Section FallDecoupled.
         [subst; intuition | right; inversion 1; contradiction]).
   Admitted.
 
+  Require Import Monad.
+
   Definition fall_decoupled 
            : marked_graph (event even odd) transitions_FD :=
   {| mg_triples := 
-     let eo_f := fun (E : even) (O : odd) pf =>
+     let eo_f := fun (EO : even * odd) => let (E,O) := EO in
                      [ (Rise (Even E), Even_fall E, Fall (Even E))
                      ; (Fall (Even E), Even_rise E, Rise (Even E))
-                     ; (Rise (Even E), Even_rise_odd_rise E O pf, Rise (Odd O))
-                     ; (Fall (Odd O), Odd_fall_even_rise E O pf, Rise (Even E))
+                     ; (Rise (Even E), Even_rise_odd_rise E O (*pf*), Rise (Odd O))
+                     ; (Fall (Odd O), Odd_fall_even_rise E O (*pf*), Rise (Even E))
                      ; (Rise (Odd O), Odd_fall O, Fall (Odd O))
                      ]
      in
-     let oe_f := fun (O : odd) (E : even) pf =>
+     let oe_f := fun (OE : odd * even) => let (O,E) := OE in
                      [ (Rise (Odd O), Odd_fall O, Fall (Odd O))
                      ; (Fall (Odd O), Odd_rise O, Rise (Odd O))
-                     ; (Rise (Odd O), Odd_rise_even_rise O E pf, Rise (Even E))
-                     ; (Fall (Even E), Even_fall_odd_rise O E pf, Rise (Odd O))
+                     ; (Rise (Odd O), Odd_rise_even_rise O E (*pf*), Rise (Even E))
+                     ; (Fall (Even E), Even_fall_odd_rise O E (*pf*), Rise (Odd O))
                      ; (Rise (Even E), Even_fall E, Fall (Even E))
                      ]
-     in flat_map_proof (even_odd_neighbors c) eo_f
-     ++ flat_map_proof (odd_even_neighbors c) oe_f
+     in flat_map eo_f (even_odd_neighbors c)
+     ++ flat_map oe_f (odd_even_neighbors c)
    ; mg_init := fun p => match p with
-                | Even_rise_odd_rise _ _ _ => 1
+                | Even_rise_odd_rise _ _ => 1
                 | Even_fall _ => 1
                 | Odd_rise _ => 1
                 | _ => 0
                 end
    |}.
 
+
+Inductive is_enabled_FD : event even odd -> marking transitions_FD -> Prop :=
+| Even_fall_enabled E m :
+  0 < m (Even_fall E) ->
+  is_enabled_FD (Fall (Even E)) m
+| Even_rise_enabled E m :
+  (forall O (pf : In (O,E) (odd_even_neighbors c)),
+          0 < m (Odd_rise_even_rise O E)) ->
+  (forall O (pf : In (E,O) (even_odd_neighbors c)),
+          0 < m (Even_rise E)) ->
+  (forall O (pf : In (E,O) (even_odd_neighbors c)),
+          0 < m (Odd_fall_even_rise E O)) ->
+  is_enabled_FD (Rise (Even E)) m
+| Odd_fall_enabled O m :
+  0 < m (Odd_fall O) ->
+  is_enabled_FD (Fall (Odd O)) m
+| Odd_rise_enabled O m :
+  (forall E (pf : In (E,O) (even_odd_neighbors c)),
+          0 < m (Even_rise_odd_rise E O)) ->
+  (forall E (pf : In (O,E) (odd_even_neighbors c)),
+          0 < m (Odd_rise O)) ->
+  (forall E (pf : In (O,E) (odd_even_neighbors c)),
+          0 < m (Even_fall_odd_rise O E)) ->
+  is_enabled_FD (Rise (Odd O)) m
+.
+
+
+
+Lemma FD_is_enabled_equiv : forall e m,
+    is_enabled_FD e m -> is_enabled fall_decoupled e m.
+Proof.
+  destruct e as [[O | E] | [O | E]];
+    intros m; inversion 1; subst;
+    apply forallb_forall; intros T pf_in;
+    apply PeanoNat.Nat.ltb_lt;
+
+    unfold preset in pf_in;
+    inversion_In; simpl in *.
+
+  * compare e (Rise (Odd O) : event even odd); inversion_In. 
+    repeat case_In; eauto.
+  * compare e (Rise (Even E) : event even odd); inversion_In. 
+    repeat case_In; eauto.
+  * compare e (Fall (Odd O) : event even odd); inversion_In. 
+    repeat case_In; eauto.
+  * compare e (Fall (Even E) : event even odd); inversion_In. 
+    repeat case_In; eauto.
+Qed.
+  
+Lemma is_enabled_RD_equiv : forall e m,
+    is_enabled fall_decoupled e m ->
+    is_enabled_FD e m.
+Proof.
+  intros e m Henabled.
+  unfold is_enabled, enabled in Henabled.
+  destruct e as [[O | E] | [O | E]].
+  * constructor; intros E pfE.
+    + apply PeanoNat.Nat.ltb_lt.
+      destruct (forallb_forall (fun t => 0 <? m t) (preset _ fall_decoupled (Rise (Odd O))))
+        as [Hforall _].
+      specialize (Hforall Henabled).
+      apply Hforall.
+      unfold preset. unfold fall_decoupled. simpl.
+      apply in_flat_map.
+      exists (Rise (Even E), Even_rise_odd_rise E O, Rise (Odd O)).
+      split.
+      2:{ simpl. rewrite eqb_eq. simpl. auto. }
+      apply in_or_app.
+      left.
+      apply in_flat_map.
+      exists (E,O). split; auto.
+      simpl. auto.
+  (* good *)
+Admitted.
+
+
+
+
+  Lemma sync_eval_S : forall n l st,
+    (forall l', neighbor _ _ c l' l ->
+                 st l' = match l with
+                        | Even _ => sync_eval c init_st n l'
+                        | Odd _  => sync_eval c init_st (S n) l'
+                        end) ->
+    sync_eval c init_st (S n) l = next_state c st l.
+  Proof.
+    intros n [O | E] st Hst; subst.
+      + simpl. apply f_equal. apply functional_extensionality. intros [E HE]. simpl.
+        unfold even_state. simpl. rewrite Hst; auto. constructor; auto.
+      + simpl. apply f_equal. apply functional_extensionality. intros [O HO]. simpl.
+        unfold odd_state. simpl. rewrite Hst; auto. constructor; auto.
+  Qed.
+
+  Lemma fall_decoupled_strong : forall l b t v,
+    async_rel c init_st l b t v ->
+      forall m, {fall_decoupled}⊢ t ↓ m ->
+      forall n,
+      n = match l with
+          | Odd o => num_events (Rise (Odd o)) t
+          | Even e => 1 + num_events (Rise (Even e)) t
+          end ->
+      v = sync_eval c init_st n l.
+  Proof.
+    intros l b t v Hrel.
+    induction Hrel; intros m Hm n Hn.
+    * (* Because l is opaque in the initial marking, l must be odd. *)
+      inversion Hm; subst.
+      destruct l as [O | E].
+      2:{ contradict H. rewrite H2; [inversion 1 | ].
+          apply FD_is_enabled_equiv.
+          constructor; auto.
+      }
+      simpl. reflexivity.
+    * (* l is transparent *)
+      rewrite H2.
+
+    (* n > 0 *)
+    destruct n as [|n].
+    { subst. destruct l as [O | E].
+        2:{ inversion Hn. }
+        (* since the initial state of odd latches are opaque *)
+        admit.
+    }
+
+    erewrite sync_eval_S; auto.
+    intros l' Hl'. 
+    erewrite H1; eauto.
+    
+    inversion Hl'; subst.
+    { assert (Hfact : transparent t (Odd O) = true ->
+                      num_events (Rise (Odd O)) t = 1+ num_events (Rise (Even E)) t)
+        by admit.
+      rewrite Hfact in Hn; auto.
+      inversion Hn.
+      reflexivity.
+    }
+    { assert (Hfact : transparent t (Even E) = true ->
+                      num_events (Rise (Even E)) t = num_events (Rise (Odd O)) t)
+        by admit.
+      inversion Hn.
+      rewrite Hfact; auto.
+    }
+
+  * inversion Hm; subst.
+    simpl in H. compare (Rise l) e.
+    erewrite IHHrel; eauto.
+    { destruct l; simpl; reduce_eqb; reflexivity. }
+
+  * 
+    destruct n as [|n].
+    { simpl in Hn. subst. destruct l as [O | E].
+        2:{ inversion Hn. }
+        (* since the initial state of odd latches are opaque *)
+        simpl in Hn.
+        rewrite sync_eval_odd_0.
+
+        inversion Hm; subst.
+        (* O- is enabled, but O+ has not yet occurred, this is a contradiction since O starts out low. *)
+        admit.
+    }
+
+    erewrite sync_eval_S; eauto.
+    intros l' Hl'.
+
+    inversion Hm; subst.
+
+    erewrite H1; eauto.
+    
+    (* since Fall l is enabled *)
+     inversion Hl'; subst.
+     { rewrite Hn.
+       f_equal. simpl.
+       assert (Hfact : transparent t (Odd O) = true ->
+                      num_events (Rise (Odd O)) t = 1+ num_events (Rise (Even E)) t)
+        by admit.
+       rewrite Hfact; auto.
+       { (* since O- is enabled in t, O must be transparent in t *) admit. }
+     }
+    { inversion Hn; subst.
+      assert (Hfact : transparent t (Even E) = true ->
+                      num_events (Rise (Even E)) t = num_events (Rise (Odd O)) t)
+        by admit.
+      rewrite <- Hfact; auto.
+      { (* since E- is enabled in t, E must be transparent in t *) admit. }
+Admitted.    
+
+
+
+(*
+
+Lemma rise_enabled_even_odd : forall t m O E,
+    {fall_decoupled}⊢ t ↓ m ->
+    is_enabled fall_decoupled (Rise (Odd O)) m ->
+    In (E,O) (even_odd_neighbors c) ->
+    num_events (Rise (Even E)) t = num_events (Rise (Odd O)) t.
+Admitted.
+
+Lemma rise_enabled_odd_even : forall t m O E,
+    {fall_decoupled}⊢ t ↓ m ->
+    is_enabled fall_decoupled (Rise (Even E)) m ->
+    In (O,E) (odd_even_neighbors c) ->
+    num_events (Rise (Odd O)) t = 1+num_events (Rise (Even E)) t.
+Admitted.
+
+Lemma async_rel_transparent : forall l b t v,
+    async_rel c init_st l b t v ->
+    forall e,
+    e <> Rise l ->
+    e <> Fall l ->
+    transparent (next_trace e t) l = true ->
+    async_rel c init_st l true (next_trace e t) v.
+Proof.
+  intros l b t v Hrel.
+Import FE_Tactics.
+  induction Hrel; intros e0 Hrise Hfall Ht; reduce_transparent.
+  + econstructor; eauto.
+    { reduce_transparent. auto. }
+    intros l' [ | ] Hneighbor.
+    ++ (* true *)
+      compare e0 (Rise l').
+  Admitted.    
+*)
+
+
+(*
+
+Lemma event_fall_invariant_fd : forall l b t v,
+    async_rel c init_st l b t v ->
+    forall e,
+    e <> Rise l ->
+    forall m, {fall_decoupled}⊢ next_trace e t ↓ m ->
+    async_rel c init_st l (transparent (next_trace e t) l) (next_trace e t) v.
+Proof.
+    intros.
+    simpl. unfold update_transparency_predicate.
+    reduce_eqb.
+    compare (Fall l) e.
+    { (* e = Fall l *)
+      econstructor; eauto.
+      simpl. unfold update_transparency_predicate.
+      reduce_eqb. auto.
+    }
+
+    compare (transparent t l) false.
+    { rewrite e0. econstructor; eauto.
+      simpl. unfold update_transparency_predicate.
+      reduce_eqb; auto.
+    }
+
+
+Qed.
+
+    *)
+
+
+
+Proof.
+  intros l e t v Hrel.
+Require Import Coq.Program.Equality.
+  remember (next_trace e t) as t'.
+  revert e t Heqt'.
+  induction Hrel as [? ? Hopaque | ? ? ? ? Htransparent ? | ? ? ? ? Hopaque ?];
+    intros e' t' Heqt' Hneq m Hm; subst.
+  * inversion Heqt'.
+  * inversion Hm; subst.
+    simpl in Htransparent.
+    unfold update_transparency_predicate in Htransparent.
+    reduce_eqb.
+    compare (Fall l) e'.
+    eapply async_transparent; auto.
+    intros l' Hneighbor.
+    assert (transparent (next_trace e' t') l' = false).
+    { simpl. unfold update_transparency_predicate.
+      (* since e' is enabled in m0 ~ t', if e' = Rise l', then l must have been
+      opaque, which is a contradiction. *)
+      (* if e' = Fall l', then we're good. *)
+      compare (Rise l') e'.
+      { contradict Htransparent. admit. }
+      compare (Fall l') e'; [auto | ].
+      admit (* induction? *).
+    }
+    
+
+    eapply H0; eauto.
+
+
+
+    apply Htransparent.
+
+ as [? ? Hopaque | ? ? ? Htransparent ? | ? ? ? ? Hopaque Hrel]; intros e0 He0.
+  + 
+
+(*    
+Inductive sync_rel : nat -> latch even odd -> value -> Prop :=
+| Sync_odd_0 (O : odd) :  sync_rel 0 (Odd O) (init_st (Odd O)) (* Odd O ⇓^{0} init_st(Odd O)*)
+| Sync_odd_S (O : odd) (n : nat) (st0 : state (latch even odd)) :
+    (forall (E : even) (pf : In (E,O) (even_odd_neighbors c)), 
+            sync_rel (S n) (Even E) (st0(Even E))) ->
+    sync_rel (S n) (Odd O) (next_state c st0 (Odd O))
+| Sync_even_S (E : even) (n : nat) (st0 : state (latch even odd)) :
+    (forall (O : odd) (pf : In (O,E) (odd_even_neighbors c)), 
+            sync_rel n (Odd O) (st0(Odd O))) ->
+    sync_rel (S n) (Even E) (next_state c st0 (Even E))
+.
+
+Fixpoint length_trace (t : trace even odd) : nat :=
+  match t with
+  | empty_trace _ => 0
+  | next_trace _ t' => 1 + length_trace t'
+  end.
+*)
+
+ Lemma event_fall_invariant_fd : forall n l v,
+    sync_rel n l v ->
+    forall t st st' e,
+    c ⊢ init_st ⇒t⇒ st ->
+    async_step c (transparent t) st e st' ->
+    e <> Rise l ->
+    transparent (next_trace e t) l = true ->
+    st'(l) = st(l).
+  Proof.
+    intros n l v Hrel.
+    induction Hrel; intros t st st' e Hst Hstep He Htransparent.
+    * simpl in Htransparent. unfold update_transparency_predicate in *.
+      reduce_eqb.
+      compare (Fall (Odd O) : event even odd) e; [contradict Htransparent; auto | ].
+      destruct Hstep.
+      
+
+    * simpl in Htransparent. unfold update_transparency_predicate in *.
+      reduce_eqb.
+      
+
+  Lemma event_disjoint_fd : forall n l v,
+    sync_rel n l v ->
+    forall t m st st',
+    {fall_decoupled}⊢ t ↓ m ->
+    n <= length_trace t ->
+    c ⊢ st ⇒t⇒st' ->
+    disjoint l t ->
+    transparent t l = true ->
+    st'(l) = st(l).
+  Proof.
+    intros n l v Hsync.
+    induction Hsync; intros t m st st' Hm Hlen Hst Hdisjoint Htransparent.
+    * contradict Htransparent. Search transparent Odd. admit (* true *).
+    * erewrite eval_transparent; eauto.
+      admit (* because O is disjoint from t and transaprent in t, it must also be transparent in the initial marking, which is a contradiction. *).
+    * erewrite eval_transparent; eauto.
+      transitivity (next_state c st (Even E)).
+      2:{ (* because E is disjoint from t and transaprent in t, it must also be transaprent in the initial marking. *) admit. }
+
+      simpl. apply f_equal. unfold odd_state.
+      apply functional_extensionality. intros [O Hpf]. simpl.
+
+      assert (
+
+
+    {fall_decoupled}⊢ t ↓ m ->
+    c ⊢ st ⇒t⇒ st' ->
+    disjoint l t ->
+    st'(l) = st(l).
+  Proof.
+    intros t m st st' l Hm Hst Hdisjoint.
+    revert m st st' Hm Hst.
+    induction Hdisjoint; intros m st st' Hm Hst.
+    *  inversion Hst; auto.
+    * 
+
+    induction t as [P | e t]; intros m st st' l Hm Hst Hdisjoint.
+    * inversion Hst. reflexivity.
+    * inversion Hst as [ | e0 t0  st0 st'0 Hst' Hopaque Htransparent]; subst.
+      inversion Hdisjoint as [ | l0 e0 t0 e_neq_l Hpred Hdisjoint']; subst.
+      inversion Hm as [ | e0 m' m0' t0 Henabled Hfire Hm']; subst.
+      
+
+  Admitted.
+
+  Lemma event_fall_invariant_fd : forall t st l st',
+    c ⊢ init_st ⇒t⇒ st ->
+    async_step c (transparent t) st (Fall l) st' ->
+    forall l', st'(l') = st(l').
+  Proof.
+(*
+    induction t as [P | e t]; intros st l st' Hst [Hopaque Htransparent] l'.
+    * (* t = [] *)
+      inversion Hst as [P0 Htransparencies | ]; subst.
+     
+
+    destruct ((update_transparency_predicate (Fall l) P) l')
+      eqn:Hl';
+      unfold update_transparency_predicate in Hl';
+      simpl in Hl'.
+    + (* l is transparent *)
+      compare l l'; [contradict Hl'; auto | ].
+      rewrite eqb_neq in Hl'; [ | inversion 1; subst; contradiction].
+      
+     
+
+    destruct ((update_transparency_predicate (Fall l) (transparent t)) l')
+      eqn:Hl'.
+    * (* l' is transparent *)
+
+      rewrite Htransparent; auto.
+
+      unfold update_transparency_predicate in Hl'.
+      simpl in Hl'.
+      assert (Fall l' <> Fall l).
+      { inversion 1; subst. rewrite eqb_eq in Hl'. inversion Hl'. }
+      rewrite eqb_neq in Hl'; auto.
+
+      erewrite (eval_transparent _ _ t st); eauto.
+      unfold next_state.
+
+      admit (* need induction? *).
+    * (* l' is opaque *)
+      unfold update_transparency_predicate in Hl'.
+      simpl in Hl'.
+Existing Instance latch_eq_dec.
+      destruct (Dec l' l).
+      ** subst.
+         erewrite Hopaque; eauto.
+      ** rewrite eqb_neq in Hl'; [ | inversion 1; contradiction].
+         rewrite Hopaque; auto.
+         unfold update_transparency_predicate. simpl.
+         rewrite eqb_neq; auto.
+         inversion 1; contradiction.
+*)
+  Admitted.
 
 
   Lemma event_rise_invariant_fd : forall t m st st' l,
@@ -91,25 +522,13 @@ Section FallDecoupled.
     destruct e as [l' | l'].
     * eapply event_rise_invariant_fd; eauto.
       inversion 1; subst; contradiction.
-    * eapply event_fall_invariant; eauto.
+    * eapply event_fall_invariant_fd; eauto.
   Qed.
 
 
 
-Lemma rise_enabled_even_odd : forall t m O E,
-    {fall_decoupled}⊢ t ↓ m ->
-    is_enabled fall_decoupled (Rise (Odd O)) m ->
-    In (E,O) (even_odd_neighbors c) ->
-    num_events (Rise (Even E)) t = num_events (Rise (Odd O)) t.
-Admitted.
 
-Lemma rise_enabled_odd_even : forall t m O E,
-    {fall_decoupled}⊢ t ↓ m ->
-    is_enabled fall_decoupled (Rise (Even E)) m ->
-    In (O,E) (odd_even_neighbors c) ->
-    num_events (Rise (Odd O)) t = 1+num_events (Rise (Even E)) t.
-Admitted.
-
+Opaque sync_eval.
   Lemma fall_decoupled_strong : 
     forall t,
       forall m, {fall_decoupled}⊢ t ↓ m ->
@@ -121,23 +540,18 @@ Admitted.
       intros m Hm st Heval;
       split; intros l.
     * (* base case, odd *)
-      simpl. inversion Heval; subst. rewrite sync_eval_odd_0. reflexivity.
+      simpl. inversion Heval; subst. reflexivity.
     * (* base case, even *)
       simpl. inversion Heval; subst.
       erewrite eval_transparent; eauto.
-      { simpl. rewrite sync_eval_even.
-        f_equal.
-        unfold odd_state.
-        apply functional_extensionality.
-        intros [O Ho]. simpl.
-        rewrite sync_eval_odd_0. reflexivity.
+      { simpl. rewrite sync_eval_even. reflexivity.
       }
       { simpl.
         inversion Hm as [P0 Hopaque Htransparent | ]; clear H P0; rewrite <- H2 in *; clear m H2.
         apply Htransparent.
 
-        (* apply is_enabled_fd. *)
-        admit (* LEMMA *).
+        apply FD_is_enabled_equiv.
+        constructor; auto.
       }
     * (* inductive case, odd *)
 
@@ -173,7 +587,6 @@ Admitted.
 
       rewrite eqb_neq; auto.
     
-
       rewrite (event_invariant_neq t m st' st e); eauto.
       2:{ split; auto. }
 
@@ -221,7 +634,7 @@ Admitted.
       destruct (IHt m Hconsistent' st' Heval') as [_ IH].
       rewrite IH.
       reflexivity.
-  Admitted.
+  Qed.
       
 
 Lemma num_events_odd_opaque : forall t st m O,
