RiseDecoupled.v
@@ -1,3 +1,4 @@
+Require Import Base.
 Require Import FlowEquivalence.
 Require Import List.
 Import ListNotations.
@@ -6,7 +7,6 @@ Open Scope list_scope.
 
 
 Require Import PeanoNat.
-Infix "<?" := (Nat.ltb).
 
 Existing Instance event_eq_dec.
 Existing Instance latch_eq_dec.
@@ -29,14 +29,39 @@ Section RiseDecoupled.
   | Odd_fall  (O : odd) : transitions_RD
   | Odd_rise  (O : odd) : transitions_RD
   (* E- → O- *)
-  | Even_odd_fall (E : even) (O : odd) : In (E,O) (even_odd_neighbors c) -> transitions_RD
+  | Even_odd_fall (E : even) (O : odd) : (*In (E,O) (even_odd_neighbors c) ->*) transitions_RD
   (* O- → E+ *)
-  | Odd_even_rise (E : even) (O : odd)  : In (E,O) (even_odd_neighbors c) -> transitions_RD
+  | Odd_even_rise (E : even) (O : odd)  : (*In (E,O) (even_odd_neighbors c) ->*) transitions_RD
   (* E- → O+ *)
-  | Even_odd_rise (O : odd)  (E : even) : In (O,E) (odd_even_neighbors c) -> transitions_RD
+  | Even_odd_rise (O : odd)  (E : even) : (*In (O,E) (odd_even_neighbors c) ->*) transitions_RD
   (* O- → E- *)
-  | Odd_even_fall (O : odd)  (E : even) : In (O,E) (odd_even_neighbors c) -> transitions_RD
+  | Odd_even_fall (O : odd)  (E : even) : (*In (O,E) (odd_even_neighbors c) ->*) transitions_RD
   .
+
+
+  Definition input_RD (t : transitions_RD) : event even odd :=
+    match t with
+    | Even_fall E => Rise (Even E)
+    | Even_rise E => Fall (Even E)
+    | Odd_fall o => Rise  (Odd o)
+    | Odd_rise o => Fall (Odd o)
+    | Even_odd_fall E o => Fall (Even E)
+    | Odd_even_rise E o => Fall (Odd o)
+    | Even_odd_rise o E => Fall (Even E)
+    | Odd_even_fall o E => Fall (Odd o)
+    end.
+  Definition output_RD (t : transitions_RD) : event even odd :=
+    match t with
+    | Even_fall E => Fall (Even E)
+    | Even_rise E => Rise (Even E)
+    | Odd_fall o =>  Fall (Odd o)
+    | Odd_rise o =>  Rise (Odd o)
+    | Even_odd_fall E o => Fall (Odd o)
+    | Odd_even_rise E o => Rise (Even E)
+    | Even_odd_rise o E => Rise (Odd o)
+    | Odd_even_fall o E => Fall (Even E)
+    end.
+
 
 
   Instance eqdecRD : eq_dec transitions_RD.
@@ -48,35 +73,36 @@ Section RiseDecoupled.
         [subst; intuition | right; inversion 1; contradiction]);
       try (destruct (Dec O O0) as [HB | HB];
         [subst; intuition | right; inversion 1; contradiction]).
+(*    * rewrite (proof_irrelevance _ i i0). intuition.
     * rewrite (proof_irrelevance _ i i0). intuition.
     * rewrite (proof_irrelevance _ i i0). intuition.
     * rewrite (proof_irrelevance _ i i0). intuition.
-    * rewrite (proof_irrelevance _ i i0). intuition.
+*)
   Qed.
 
 
   Definition rise_decoupled 
            : marked_graph (event even odd) transitions_RD :=
   {| mg_triples := 
-     let eo_f := fun (A : even) (B : odd) pf =>
-                     [ (Rise (Even A), Even_fall A, Fall (Even A))
-                     ; (Fall (Even A), Even_odd_fall A B pf, Fall (Odd B))
-                     ; (Fall (Odd B), Odd_even_rise A B pf, Rise (Even A))
-                     ; (Rise (Odd B), Odd_fall B, Fall (Odd B))
-                     ; (Fall (Odd B), Odd_rise B, Rise (Odd B))
+     let eo_f := fun (eo : even * odd) => let (E,O) := eo in
+                     [ (Rise (Even E), Even_fall E, Fall (Even E))
+                     ; (Fall (Even E), Even_odd_fall E O, Fall (Odd O))
+                     ; (Fall (Odd O), Odd_even_rise E O, Rise (Even E))
+                     ; (Rise (Odd O), Odd_fall O, Fall (Odd O))
+                     ; (Fall (Odd O), Odd_rise O, Rise (Odd O))
                      ]
      in
-     let oe_f := fun (A : odd) (B : even) pf =>
-                     [ (Rise (Odd A), Odd_fall A, Fall (Odd A))
-                     ; (Fall (Odd A), Odd_even_fall A B pf, Fall (Even B))
-                     ; (Fall (Even B), Even_odd_rise A B pf, Rise (Odd A))
-                     ; (Rise (Even B), Even_fall B, Fall (Even B))
-                     ; (Fall (Even B), Even_rise B, Rise (Even B))
+     let oe_f := fun (oe : odd * even) => let (O,E) := oe in
+                     [ (Rise (Odd O), Odd_fall O, Fall (Odd O))
+                     ; (Fall (Odd O), Odd_even_fall O E, Fall (Even E))
+                     ; (Fall (Even E), Even_odd_rise O E, Rise (Odd O))
+                     ; (Rise (Even E), Even_fall E, Fall (Even E))
+                     ; (Fall (Even E), Even_rise E, Rise (Even E))
                      ]
-     in flat_map_proof (even_odd_neighbors c) eo_f
-     ++ flat_map_proof (odd_even_neighbors c) oe_f
+     in flat_map eo_f (even_odd_neighbors c)
+     ++ flat_map oe_f (odd_even_neighbors c)
    ; mg_init := fun p => match p with 
-                         | Odd_even_fall _ _ _ => 1
+                         | Odd_even_fall _ _ => 1
                          | Even_fall _ => 1
                          | Odd_rise _ => 1
                          | _ => 0
@@ -88,68 +114,102 @@ Section RiseDecoupled.
 Open Scope nat_scope.
 Inductive is_enabled_RD : event even odd -> marking transitions_RD -> Prop :=
 | Even_fall_enabled E m :
-  0 < m (Even_fall E) ->
+  (forall O (pf : In (E,O) (even_odd_neighbors c)),
+          0 < m (Even_fall E)) ->
   (forall O (pf : In (O,E) (odd_even_neighbors c)),
-          0 < m (Even_odd_rise O E pf)) ->
+          0 < m (Even_fall E)) ->
+  (forall O (pf : In (O,E) (odd_even_neighbors c)),
+          0 < m (Odd_even_fall O E)) ->
   is_enabled_RD (Fall (Even E)) m
 | Even_rise_enabled E m :
   (forall O (pf : In (O,E) (odd_even_neighbors c)),
           0 < m (Even_rise E)) ->
   (forall O (pf : In (E,O) (even_odd_neighbors c)),
-          0 < m  (Odd_even_rise E O pf)) ->
+          0 < m  (Odd_even_rise E O)) ->
   is_enabled_RD (Rise (Even E)) m
 | Odd_fall_enabled O m :
-  0 < m (Odd_fall O) ->
   (forall E (pf : In (E,O) (even_odd_neighbors c)),
-          0%nat < m (Even_odd_fall E O pf)) ->
+          0 < m (Odd_fall O)) ->
+  (forall E (pf : In (O,E) (odd_even_neighbors c)),
+          0 < m (Odd_fall O)) ->
+  (forall E (pf : In (E,O) (even_odd_neighbors c)),
+          0 < m (Even_odd_fall E O)) ->
   is_enabled_RD (Fall (Odd O)) m
 | Odd_rise_enabled O m :
   (forall E (pf : In (E,O) (even_odd_neighbors c)),
           0 < m (Odd_rise O)) ->
   (forall E (pf : In (O,E) (odd_even_neighbors c)),
-          0 < m (Even_odd_rise O E pf)) ->
+          0 < m (Even_odd_rise O E)) ->
   is_enabled_RD (Rise (Odd O)) m
 .
 Lemma RD_is_enabled_equiv : forall e m,
     is_enabled_RD e m -> is_enabled rise_decoupled e m.
 Proof.
   destruct e as [[O | E] | [O | E]];
-    intros m; intros H.
-  * unfold is_enabled. unfold enabled. apply forallb_forall.
-    intros T pf_in.
-    inversion H; subst.
-    apply PeanoNat.Nat.ltb_lt.
-    unfold preset in pf_in.
-    unfold rise_decoupled in pf_in. simpl in pf_in.
-    apply in_flat_map in pf_in.
-    destruct pf_in as [[[e1 T0] e2] [pf_in1 pf_in2]].
-    simpl in pf_in2.
-    destruct (Dec e2 (Rise (Odd O)));
-      [ subst; rewrite eqb_eq in pf_in2; inversion pf_in2;
-        [ subst; clear pf_in2 | contradiction]
-        | rewrite eqb_neq in pf_in2; [contradiction | assumption] ].
-    apply in_app_or in pf_in1.
-    destruct pf_in1 as [pf_in1 | pf_in1].
-    ** apply in_flat_map_proof' in pf_in1.
-       destruct pf_in1 as [E1 [O1 [pf1 pf]]].
-       simpl in pf.
-       destruct pf as [pf | [pf | [pf | [pf | [pf | pf]]]]];
-         try (inversion pf); subst; clear pf.
-       eapply H1; eauto.
-    ** apply in_flat_map_proof' in pf_in1.
-       destruct pf_in1 as [E1 [O1 [pf1 pf]]].
-       simpl in pf.
-       destruct pf as [pf | [pf | [pf | [pf | [pf | pf]]]]];
-         try (inversion pf).
-       subst.
-       apply H2.
-(* good *)
-Admitted.
+    intros m; inversion 1; subst;
+    apply forallb_forall; intros T pf_in;
+    apply PeanoNat.Nat.ltb_lt;
+
+    unfold preset in pf_in;
+    inversion_In; simpl in *.
+
+  * compare e (Rise (Odd O) : event even odd); inversion_In. 
+    repeat case_In; eauto.
+  * compare e (Rise (Even E) : event even odd); inversion_In. 
+    repeat case_In; eauto.
+  * compare e (Fall (Odd O) : event even odd); inversion_In. 
+    repeat case_In; eauto.
+  * compare e (Fall (Even E) : event even odd); inversion_In. 
+    repeat case_In; eauto.
+Qed.
   
+
+  Ltac in_preset := 
+  match goal with
+  | [ |- In ?t (preset _ rise_decoupled ?e) ] => apply in_flat_map; exists (input_RD t, t, e);
+    split; [ | simpl; reduce_eqb; simpl; auto ];
+    apply in_or_app
+  end;
+  try (left;
+       repeat match goal with
+       | [ |- In (_, ?t _, _) (flat_map _ _) ] => apply in_flat_map
+       | [ E : even , O : odd |- exists x : even * odd, _ ] => exists (E,O)
+       | [ E : even , O : odd |- exists x : odd * even, _ ] => exists (E,O)
+       end; intuition; fail);
+  try (right;
+       repeat match goal with
+       | [ |- In (_, ?t _, _) (flat_map _ _) ] => apply in_flat_map
+       | [ E : even , O : odd |- exists x : even * odd, _ ] => exists (E,O)
+       | [ E : even , O : odd |- exists x : odd * even, _ ] => exists (O,E)
+       end; intuition; fail).
+
 Lemma is_enabled_RD_equiv : forall e m,
     is_enabled rise_decoupled e m ->
     is_enabled_RD e m.
-Admitted.
+Proof.
+  intros e m Henabled.
+  unfold is_enabled, enabled in *.
+  assert (H : forall t, In t (preset _ rise_decoupled e) -> 0 <? m t = true).
+  { apply forallb_forall; auto. }
+  clear Henabled.
+  assert (Henabled : forall t, In t (preset _ rise_decoupled e) -> 0 < m t).
+  { intros.
+    apply Nat.ltb_lt.
+    apply H. auto.
+  }
+  clear H.
+  
+  destruct e as [[O | E] | [O | E]].
+  * constructor; intros E pfE;
+      apply Henabled; in_preset.
+  * constructor; intros O pfO;
+      apply Henabled; in_preset.
+  * constructor; intros E pfE;
+      apply Henabled; in_preset.
+  * constructor; intros O pfO;
+      apply Henabled; in_preset.
+Qed.
+
 
 Lemma rise_decoupled_init_even : forall P E m,
     {rise_decoupled}⊢ empty_trace P ↓ m ->
@@ -168,15 +228,12 @@ Proof.
           inversion H as [ | H0]; [subst | inversion H0]; clear H.
           apply in_app_or in HT.
           destruct HT as [HT | HT].
-          ++ apply in_flat_map_proof' in HT.
-             destruct HT as [E0 [O0 [pf0 HT]]].
-             simpl in HT.
-             repeat (destruct HT as [HT | HT]; [ inversion HT; subst; auto | ]); inversion HT.
-          ++ apply in_flat_map_proof' in HT.
-             destruct HT as [E0 [O0 [pf0 HT]]].
-             simpl in HT.
-             repeat (destruct HT as [HT | HT]; [ inversion HT; subst; auto | ]); inversion HT.
+          ++ inversion_In. repeat (case_In; auto).
+          ++ inversion_In. repeat (case_In; auto). 
 Qed.
+
+
+
 
 
 Lemma fall_enabled_even_opaque : forall s m O E,
@@ -206,6 +263,133 @@ Lemma fall_enabled_odd_even : forall s m O E,
     In (O,E) (odd_even_neighbors c) ->
     num_events (Fall (Odd O)) s = num_events (Fall (Even E)) s.
 Admitted.
+
+
+
+
+Require Import Coq.Program.Equality.
+Lemma rel_fe : forall l b t v,
+    async_rel c init_st l b t v ->
+    b = false ->
+    forall m,
+    {rise_decoupled}⊢ t ↓ m ->
+    v = sync_eval c init_st (num_events (Fall l) t) l.
+Proof.
+  intros l b t v Hrel.
+  
+  induction Hrel; intros Hb m Hm; find_contradiction.
+  * destruct l as [O | E].
+    (* l must be odd *)
+    2:{ contradict H. inversion Hm as [P' Htransparent Hopaque | ].
+        rewrite Hopaque; [inversion 1 | ].
+        apply RD_is_enabled_equiv.
+        simpl.
+        constructor; intros; auto.
+    }
+    simpl. reflexivity.
+  * inversion Hm as [ | e0 m0 ? t' Henabled Hfire Hm']; subst; rename m0 into m.
+    simpl in *.
+    compare (Rise l) e.
+    eapply IHHrel; eauto.
+
+  * inversion Hm as [ | e0 m0 ? t' Henabled Hfire Hm']; subst; rename m0 into m.
+    simpl in *.
+    reduce_eqb.
+    set (st' := fun n => fun l' => match l with
+                          | Even _ => sync_eval c init_st n l'
+                          | Odd _  => sync_eval c init_st (S n) l'
+                          end).
+    assert (Hstep : forall n, sync_eval c init_st (S n) l = next_state c (st' n) l).
+    { destruct l; intros n; simpl.
+      + apply f_equal. apply functional_extensionality. intros [E HE]. simpl.
+        unfold even_state. simpl. reflexivity.
+      + apply f_equal. apply functional_extensionality. intros [O HO]. simpl.
+        unfold even_state. simpl. reflexivity.
+    }
+    rewrite Hstep.
+    apply next_state_eq.
+    intros l' Hl'.
+    unfold st'.
+    erewrite H1; eauto.
+    2:{ inversion Hl'; subst. 
+        { eapply fall_enabled_even_opaque; eauto. }
+        { eapply fall_enabled_odd_opaque; eauto. }
+    }
+
+    { inversion Hl'; subst.
+      { erewrite fall_enabled_even_odd; eauto. }
+      { erewrite fall_enabled_odd_even; eauto. }
+    }
+        
+  Qed.
+
+
+
+  Lemma fall_enabled_transparent : forall (t : trace even odd)
+                                          (m : marking transitions_RD),
+    {rise_decoupled}⊢ t ↓ m ->
+    forall l, is_enabled rise_decoupled (Fall l) m ->
+              transparent t l = true.
+  Proof.
+    intros t m pf.
+    induction pf as [lset Htransparent Hopaque | ]; intros l Henabled.
+    * simpl. apply Hopaque.
+      assumption.
+    * apply is_enabled_RD_equiv in Henabled.
+      inversion Henabled; subst.
+      + (* Even case *)
+        simpl in *. unfold update_transparency_predicate.
+
+        compare (Rise (Even E) : event even odd) e; auto.
+        compare (Fall (Even E) : event even odd) e; auto.
+        { absurd (0 < fire (Fall (Even E)) rise_decoupled m (Even_fall E)); auto.
+          unfold fire.
+          destruct (in_dec' (Even_fall E, Fall (Even E)) (output_event rise_decoupled))
+            as [Hin | Hin].
+          2:{ contradict Hin.
+              eapply in_output_event; eauto.
+              exists (Rise (Even E)).
+              simpl.
+              apply in_or_app.
+              left.
+              apply in_flat_map.
+              eexists. split.
+              2:{ admit. }
+              admit.
+            }
+          admit (*?*). admit.
+        }
+
+        unfold fire in H2. 
+        destruct (in_dec' (Even_fall E, e) (output_event rise_decoupled)) as [H2' | H2'].
+        { admit (*contradiction.*). }
+        destruct (in_dec' (e,Even_fall E) (input_event rise_decoupled)) as [H2'' | H2''].
+        { admit (* contradiction *). }
+
+        
+        apply IHpf.
+        apply RD_is_enabled_equiv.
+        constructor; auto.
+        intros O pfO.
+        specialize (H3 O pfO).
+
+        unfold fire in H3.
+
+        destruct (in_dec' (Even_odd_rise O E, e) (output_event rise_decoupled)) as [H3' | H3'].
+        { admit (*contradiction.*). }
+        destruct (in_dec' (e,Even_odd_rise O E) (input_event rise_decoupled)) as [H3'' | H3''].
+        { admit (* contradiction *). }
+Admitted.
+
+Lemma rise_enabled_opaque :  forall {places : Set} `{Hplaces : eq_dec places}
+                                          (M : marked_graph (event even odd) places)
+                                          (t : trace even odd)
+                                          (m0 m : marking places)
+                                          (l : latch even odd),
+    {M}⊢ t ↓ m ->
+    is_enabled M (Rise l) m ->
+    transparent t l = false.
+Abort.
 
 
 
